Finished soundness for total triples [skip ci]

theories/Iris/Instance.v
@@ -1039,17 +1039,17 @@ Module IrisInstanceWithContracts
     End PartialTriple.
 
     Section TotalTriple.
-      Definition TValidContractEnvF { σs σ } (cenv : SepContractEnv) (f : 𝑭 σs σ) : iProp Σ :=
-        (⌜Wf.Acc InvokedByFunPackage (existT _ (existT _ f))⌝ -∗
+      Definition TValidContractEnvF (fuel : nat) { σs σ } (cenv : SepContractEnv) (f : 𝑭 σs σ) : iProp Σ :=
+        (⌜Wf.Acc (InvokedByFunPackage fuel) (existT _ (existT _ f))⌝ -∗
         match cenv σs σ f with
         | Some c => TValidContractSem (FunDef f) c
         | None => True
         end)%I.
-      Arguments TValidContractEnvF {σs σ} cenv f : simpl nomatch.
+      Arguments TValidContractEnvF fuel {σs σ} cenv f : simpl nomatch.
 
 
-      Definition TValidContractEnvSem (cenv : SepContractEnv) : iProp Σ :=
-        ∀ σs σ (f : 𝑭 σs σ), TValidContractEnvF cenv f.
+      Definition TValidContractEnvSem (fuel : nat) (cenv : SepContractEnv) : iProp Σ :=
+        ∀ σs σ (f : 𝑭 σs σ), TValidContractEnvF fuel cenv f.
 
         Definition TForeignSem :=
           ∀ (Δ : PCtx) (τ : Ty) (f : 𝑭𝑿 Δ τ),
@@ -1080,15 +1080,15 @@ Module IrisInstanceWithContracts
           iIntros ([] _) "H"; auto. by iApply "consr".
         Qed.
         
-        Lemma iris_rule_tstm_call {Γ} (δ : CStore Γ)
+        Lemma iris_rule_tstm_call {fuel : nat} {Γ} (δ : CStore Γ)
           {Δ σ} (f : 𝑭 Δ σ) (c : SepContract Δ σ) (es : NamedEnv (Exp Γ) Δ)
           (P : iProp Σ)
           (Q : Val σ -> CStore Γ -> iProp Σ) :
           CEnv f = Some c ->
           CTriple P c (evals es δ) (fun v => Q v δ) ->
-          Wf.Acc InvokedByFunPackage (existT _ (existT _ f)) ->
-          ⊢ TValidContractEnvSem CEnv -∗
-                                         semTTriple δ P (stm_call f es) Q.
+          Wf.Acc (InvokedByFunPackage fuel) (existT _ (existT _ f)) ->
+          ⊢ TValidContractEnvSem fuel CEnv -∗
+            semTTriple δ P (stm_call f es) Q.
         Proof.
           iIntros (ceq ctrip Hwff) "cenv".
           iApply iris_rule_tstm_call_one; eauto.
@@ -1140,18 +1140,33 @@ Module IrisInstanceWithContracts
           iApply "consr". by iApply lemSem.
         Qed.
 
+        (* TODO: the user would have to provide this, we can only prove this
+                 lemma when we know the concrete functions/callgraph. *)
+        Lemma wf_InvokedByFunPackage : well_founded (InvokedByFunPackage 0).
+        Proof.
+          unfold well_founded.
+          intros caller. constructor. intros callee Hinvok.
+        Admitted. (* Admit, see note above. Leave it here to continue with the proofs below *)
+
+        Ltac solve_fuel fuel :=
+          destruct fuel;
+          cbn in *;
+          try contradiction;
+          auto.
+
         Lemma sound_tstm
           {Γ} {τ} (s : Stm Γ τ) {δ : CStore Γ}:
-          forall (PRE : iProp Σ) (POST : Val τ -> CStore Γ -> iProp Σ),
+          forall (PRE : iProp Σ) (POST : Val τ -> CStore Γ -> iProp Σ) (fuel : nat),
           TForeignSem ->
           LemmaSem ->
-          (∃ fuel, # fuel ⦃ PRE ⦄ s ; δ ⦃ POST ⦄) ->
-          (forall Δ σ (f : 𝑭 Δ σ), InvokedByStm f s -> Wf.Acc (InvokedByFunPackage) (existT _ (existT _ f))) ->
-          ⊢ (□ (∀ σs σ (f : 𝑭 σs σ), TValidContractEnvF CEnv f) -∗
+          # fuel ⦃ PRE ⦄ s ; δ ⦃ POST ⦄ ->
+          (forall Δ σ (f : 𝑭 Δ σ), InvokedByStmWithFuel fuel f s -> Wf.Acc (InvokedByFunPackage fuel) (existT _ (existT _ f))) ->
+          (* DIFF: only need to know the contract is valid for functions called by s (not for all functions such as in sound_tstm_original) *)
+          ⊢ (□ (∀ σs σ (f : 𝑭 σs σ), ⌜InvokedByStmWithFuel fuel f s⌝ -∗ TValidContractEnvF fuel CEnv f) -∗
              semTTriple δ PRE s POST)%I.
         Proof.
-          iIntros (PRE POST extSem lemSem [fuel triple] Haccf) "#vcenv".
-          iInduction triple as [x|x|x|x|x|x|x|x|x|x|x|x|x|x|x|x|x|x|x|x|x|x] "trips" forall "".
+          iIntros (PRE POST fuel extSem lemSem triple Haccf) "#vcenv".
+          iInduction triple as [x|x|x|x|x|x|x|x|x|x|x|x|x|x|x|x|x|x|x|x|x|x] "trips" forall "vcenv".
           - iApply iris_rule_tconsequence; eauto.
             now iApply "trips".
           - iApply iris_rule_tframe.
@@ -1170,73 +1185,121 @@ Module IrisInstanceWithContracts
             + iApply "trips1".
               iPureIntro.
               intros σs σ0 f Hfs.
-              eapply Haccf; now left.
+              eapply Haccf. solve_fuel fuel.
+              iIntros "!>" (σs σ0 f Hinvok).
+              iApply "vcenv". iPureIntro. solve_fuel fuel.
             + iIntros (v δ'). iApply "trips".
               iPureIntro.
               intros σs σ0 f Hfs.
-              eapply Haccf; now right.
+              eapply Haccf; solve_fuel fuel; now right.
+              iIntros "!>" (σs σ0 f Hinvok).
+              iApply "vcenv". iPureIntro. solve_fuel fuel.
           - iApply iris_rule_tstm_block.
-            now iApply "trips".
+            iApply "trips". iPureIntro. intros. apply Haccf. solve_fuel fuel.
+            iIntros "!>" (σs σ0 f Hinvok).
+            iApply "vcenv". iPureIntro. solve_fuel fuel.
           - iApply iris_rule_tstm_seq.
             + iApply "trips1".
               iPureIntro. intros Δ σ0 f Hf.
-              eapply Haccf; now left.
+              eapply Haccf; solve_fuel fuel; now left.
+              iIntros "!>" (σs σ0 f Hinvok).
+              iApply "vcenv". iPureIntro. solve_fuel fuel.
             + iIntros (v δ').
               iApply "trips".
               iPureIntro. intros Δ σ0 f Hf.
-              eapply Haccf; now right.
+              eapply Haccf; solve_fuel fuel.
+              iIntros "!>" (σs σ0 f Hinvok).
+              iApply "vcenv". iPureIntro. solve_fuel fuel.
           - iApply iris_rule_tstm_assertk.
-            iIntros (He1). now iApply "trips".
+            iIntros (He1). iApply "trips".
+            done. iPureIntro. intros. solve_fuel fuel.
+            iIntros "!>" (σs σ0 f Hinvok).
+            iApply "vcenv". iPureIntro. solve_fuel fuel.
           - iApply iris_rule_tstm_fail.
           - iApply iris_rule_tstm_read_register.
           - now iApply iris_rule_tstm_write_register.
-          - iApply iris_rule_tstm_assign. now iApply "trips".
+          - iApply iris_rule_tstm_assign. iApply "trips".
+            iPureIntro. intros. solve_fuel fuel.
+            iIntros "!>" (σs σ0 f Hinvok).
+            iApply "vcenv". iPureIntro. solve_fuel fuel.
           - iApply iris_rule_tstm_call_one; eauto.
-            iSpecialize ("vcenv" $! _ _ f (Haccf _ _ _ eq_refl)).
-            now rewrite H.
+            iSpecialize ("vcenv" $! _ _ f).
+            unfold TValidContractEnvF. rewrite H.
+            iApply "vcenv".
+            + iPureIntro. destruct fuel; cbn; now left.
+            + iPureIntro. apply Haccf. destruct fuel; cbn; now left.
           - iApply iris_rule_tstm_call_inline.
             iApply "trips".
             iPureIntro.
-            iIntros (σs σ f2 Hff2) "".
-            destruct (Haccf _ _ f eq_refl) as [Hwf].
-            now apply Hwf.
-          - iApply iris_rule_tstm_call_frame. now iApply "trips".
+            iIntros (σs σ f2 Hff2).
+            apply wf_InvokedByFunPackage_S_fuel.
+            apply Haccf. now right.
+            iIntros "!>" (σs σ f' Hinvok).
+            (* iApply "vcenv". iPureIntro. solve_fuel fuel'. *)
+            iSpecialize ("vcenv" $! _ _ f' with "[]").
+            { iPureIntro. cbn. auto. }
+            unfold TValidContractEnvF. iIntros (Haccf').
+            destruct (CEnv f') eqn:Ef'; auto.
+            iApply "vcenv". iPureIntro.
+            apply Haccf. cbn. now right.
+          - iApply iris_rule_tstm_call_frame. iApply "trips".
+            iPureIntro. intros. apply Haccf. solve_fuel fuel.
+            iIntros "!>" (σs σ f Hinvok). iApply "vcenv". iPureIntro. solve_fuel fuel.
           - now iApply iris_rule_tstm_foreign.
           - iApply iris_rule_tstm_lemmak; eauto.
             iApply "trips". iPureIntro.  intros Δ0 σ f Hf.
-            now apply Haccf.
+            apply Haccf. solve_fuel fuel.
+            iIntros "!>" (σs σ f' Hinvok).
+            iApply "vcenv". iPureIntro. solve_fuel fuel.
           - iApply iris_rule_tstm_bind.
             + iApply "trips1". iPureIntro.
-              intros. apply Haccf. now left.
+              intros. apply Haccf. solve_fuel fuel.
+              iIntros "!>" (σs σ0 f Hinvok).
+              iApply "vcenv". iPureIntro. solve_fuel fuel.
             + iIntros (v ?). iApply "trips".
-              iPureIntro. intros. apply Haccf. right. now exists v.
-          - iApply iris_rule_tstm_debugk. now iApply "trips".
+              iPureIntro. intros. apply Haccf. solve_fuel fuel. right. now exists v.
+              right. now exists v.
+              iIntros "!>" (σs σ0 f Hinvok).
+              iApply "vcenv". iPureIntro. solve_fuel fuel; right; eexists; eassumption.
+          - iApply iris_rule_tstm_debugk. iApply "trips".
+            iPureIntro. intros. apply Haccf. solve_fuel fuel.
+            iIntros "!>" (σs σ0 f Hinvok).
+            iApply "vcenv". iPureIntro. solve_fuel fuel.
           - iApply iris_rule_tstm_pattern_match.
-            + iApply "trips1". iPureIntro. intros. apply Haccf. now left.
+            + iApply "trips1". iPureIntro. intros. apply Haccf. solve_fuel fuel.
+              iIntros "!>" (σs σ0 f Hinvok). iApply "vcenv".
+              iPureIntro. solve_fuel fuel.
             + iIntros (pc δpc δΓ1). iApply "trips". iPureIntro.
-              intros. apply Haccf. right. now exists pc.
+              intros. apply Haccf. solve_fuel fuel; right; now exists pc.
+              iIntros "!>" (σs σ0 f Hinvok). iApply "vcenv".
+              iPureIntro. solve_fuel fuel; right; eexists; eassumption.
         Qed.
-        
+
         Lemma tsound :
-            TForeignSem -> LemmaSem -> ValidContractCEnv ->
-            ⊢ TValidContractEnvSem CEnv.
+          ∀ fuel,
+            TForeignSem -> LemmaSem -> TValidContractCEnv fuel ->
+            ⊢ TValidContractEnvSem fuel CEnv.
         Proof.
-          iIntros (extSem lemSem cenv σs τ f).
+          iIntros (fuel extSem lemSem cenv σs τ f).
           unfold TValidContractEnvF.
           destruct (CEnv f) eqn:Hcf; last trivial.
           iIntros "%Hwf".
           iStopProof.
           remember (existT σs (existT τ f)) as x.
-          induction Hwf as [? Hacc IH]; subst.
+          generalize dependent τ.
+          generalize dependent σs.
+          induction Hwf as [? Hacc IH].
+          intros σs τ f s Hcf ?; subst.
           rewrite /TValidContractSem. destruct s as [lvars store PRE res POST].
           iIntros "_ %ι".
           rewrite /ValidContractCEnv in cenv.
           specialize (cenv _ _ f _ Hcf ι). cbn in cenv.
-          iApply (sound_tstm extSem lemSem cenv).
-          - intros. now apply Hacc.
-          - iIntros "!>" (Δ2 σ2 f2) "%Haccf2".
-            unshelve iPoseProof (IH _ _ eq_refl) as "IH".
-        Admitted.
+          iApply (sound_tstm extSem lemSem cenv); auto.
+          iIntros "!>" (Δ2 σ2 f2 Hinvok) "%Haccf2".
+          destruct (CEnv f2) eqn:Ef2; auto.
+          iApply IH; eauto.
+          apply Hinvok.
+        Qed.
     End TotalTriple.
   End WithSailGS.
 End IrisInstanceWithContracts.
